$$ log_{a}AB= m+n = log_{a}A + log_{a}B $$

$$ AB = a^{m}a^{n} = a^{m+n} $$

$$ log_{a}A = m \text{, } log_{a}B = n \implies A=a^{m}, B=a^{n} $$

$$ a^{n} = N \implies n = log_aN $$

$$ (a^{n})^{m} = a^{n \times m} = \underbrace {a^{n}\times a^{n}\times \dots \times a^{n} \times a^{n}} _{m{\text{ times}}} = a^{\underbrace {n + n + \dots + n + n} _{m{\text{ times}}}}$$

$$ a^{n} \div a^{m} = a^{n-m} = \underbrace {a\times a\times \dots \times a\times a} _{n{\text{ times}}} \div \underbrace {a\times a\times \dots \times a\times a} _{m{\text{ times}}}$$

$$ a^{n} \times a^{m} = a^{n+m} = \underbrace {a\times a\times \dots \times a\times a} _{n{\text{ times}}} \times \underbrace {a\times a\times \dots \times a\times a} _{m{\text{ times}}}$$

$${\displaystyle a^{n}=\underbrace {a\times a\times \dots \times a\times a} _{n{\text{ times}}}}$$

$${\displaystyle a\times b=\underbrace {a + a + \dots + a + a} _{b{\text{ times}}}}$$